src/impl/TLS13.Impl.Client.fst
@@ -27,6 +27,7 @@ fn new_client_default ()
   returns c:client
   ensures CR.connection_exactly c CR.default_initial_state **
           pure (CT.client_state_correct CR.default_initial_state /\
+                CT.client_end_to_end_invariant CR.default_initial_state /\
                 CS.connection_state_sent_seal_replay_consistent
                   CR.default_initial_state /\
                 CS.connection_state_sent_seal_key_schedule_replay_consistent
@@ -40,6 +41,7 @@ fn new_client_default ()
 {
   let c = CR.new_client_default ();
   CT.lemma_initial_client_state_correct CR.default_connection_config;
+  CT.lemma_initial_client_end_to_end_invariant CR.default_connection_config;
   CS.lemma_initial_sent_seal_replay_consistent CR.default_connection_config;
   CS.lemma_initial_sent_seal_key_schedule_replay_consistent CR.default_connection_config;
   CS.lemma_initial_received_decode_replay_consistent CR.default_connection_config;
@@ -74,6 +76,11 @@ fn new_client
               (Ghost.reveal 'server_name_bytes)
               (Ghost.reveal 'trust_anchors_bytes)
               validation_time_seconds) /\
+                CT.client_end_to_end_invariant
+                  (CR.configured_initial_state
+                    (Ghost.reveal 'server_name_bytes)
+                    (Ghost.reveal 'trust_anchors_bytes)
+                    validation_time_seconds) /\
                 CS.connection_state_sent_seal_replay_consistent
                   (CR.configured_initial_state
                     (Ghost.reveal 'server_name_bytes)
@@ -108,6 +115,11 @@ fn new_client
       trust_anchors_len
       validation_time_seconds;
   CT.lemma_initial_client_state_correct
+    (CR.configured_connection_config
+      (Ghost.reveal 'server_name_bytes)
+      (Ghost.reveal 'trust_anchors_bytes)
+      validation_time_seconds);
+  CT.lemma_initial_client_end_to_end_invariant
     (CR.configured_connection_config
       (Ghost.reveal 'server_name_bytes)
       (Ghost.reveal 'trust_anchors_bytes)
